theories/lang/lang.v
@@ -512,6 +512,9 @@ Proof. intros. apply is_closed_subst with []; set_solver. Qed.
 Lemma is_closed_of_val X v : is_closed X (of_val v).
 Proof. apply is_closed_weaken_nil. induction v; simpl; auto. Qed.
 
+Lemma is_closed_to_val X e v : to_val e = Some v → is_closed X e.
+Proof. intros <-%of_to_val. apply is_closed_of_val. Qed.
+
 Lemma subst_is_closed X x es e :
   is_closed X es → is_closed (x::X) e → is_closed X (subst x es e).
 Proof.
