theories/typing/base.v
@@ -14,6 +14,9 @@ Ltac solve_typing :=
   (typeclasses eauto with lrust_typing typeclass_instances core; fail) ||
   (typeclasses eauto with lrust_typing lrust_typing_merge typeclass_instances core; fail).
 
+Lemma of_val_unlock v e : of_val v = e → of_val (locked v) = e.
+Proof. by unlock. Qed.
+
 Hint Constructors Forall Forall2 elem_of_list : lrust_typing.
 Hint Resolve
      of_val_unlock
