theories/typing/lib/panic.v
@@ -20,6 +20,6 @@ Section panic.
   Proof.
     intros E L. iApply type_fn; [solve_typing..|]. iIntros "!# *".
     inv_vec args.  iIntros (tid) "LFT HE Hna HL Hk HT /=". simpl_subst.
-    wp_value. done.
+    by iApply wp_value.
   Qed.
 End panic.
